cv_translator/eval_cake_compile_x64Lib.sml
@@ -14,7 +14,6 @@ local
     , to_livesets_def          = backend_x64Theory.to_livesets_x64_def
     , compile_cake_def         = backend_x64Theory.compile_cake_x64_def
     , compile_cake_imp         = backend_x64Theory.compile_cake_x64_thm
-    , compile_cake_explore_def = backend_x64Theory.compile_cake_explore_x64_def
     , cv_export_def            = backend_x64_cvTheory.cv_x64_export_def } : arch_thms;
 
 in
@@ -24,12 +23,6 @@ in
 
   val eval_cake_compile_x64_with_conf =
       eval_cake_compile_with_conf x64_arch_thms;
-
-  val eval_cake_compile_explore_x64 =
-      eval_cake_compile_explore x64_arch_thms;
-
-  val eval_cake_compile_explore_x64_with_conf =
-      eval_cake_compile_explore_with_conf x64_arch_thms;
 
   val eval_cake_compile_x64_general =
       eval_cake_compile_general x64_arch_thms;
